Runtime/Network/Execution/Apply.lean
@@ -1,0 +1,86 @@
+import Runtime.Network.Execution.Basic
+
+open Network
+
+structure Reaction.Output (net : Network) where
+  reactor : ReactorId net
+  reaction : reactor.class.reactionType
+  time : Time
+  raw : reaction.outputType time
+
+abbrev Reaction.Output.domain (output : Reaction.Output net) : Interface.Scheme :=
+  output.reactor.class.interface .outputs
+
+def Reaction.Output.fromRaw {reactor : ReactorId net} {reaction : reactor.class.reactionType} {time} (raw : reaction.outputType time) : Reaction.Output net :=
+  { reactor, reaction, time, raw }
+
+def Reaction.Output.events (output : Reaction.Output net) :=
+  output.raw.events.map fun event => Event.action event.time ⟨output.reactor, event.action⟩ event.value
+
+inductive Reaction.Output.LocalValue (output : Reaction.Output net) (port : output.domain.vars)
+  | independent
+  | absent
+  | present (value : output.domain.type port) -- {port : output.reaction.portEffects} (value : (output.reactor.class.interface .outputs).restrict output.reaction.portEffects |>.type port)
+
+def Reaction.Output.LocalValue.value? : LocalValue output port → Option (output.domain.type port)
+  | present value        => value
+  | independent | absent => none
+
+-- Note: This theorem is really only needed for `Reaction.Output.local`.
+def Reaction.Output.local_type_correctness {port'} : 
+  (output.reaction.portEffectsInjCoe.inv (.inl port) = some port') → 
+  (output.reactor.class.reactionOutputScheme |>.restrict output.reaction.portEffects |>.type port') = (domain output).type port :=
+  (by rw [Interface.Scheme.restrict_type, output.reaction.portEffectsInjCoe.invCoeId _ ·])
+
+def Reaction.Output.local (output : Reaction.Output net) (port : output.domain.vars) : LocalValue output port := 
+  match h : output.reaction.portEffectsInjCoe.inv (.inl port) with
+  | none => .independent
+  | some port' =>
+    match output.raw.ports port' with
+    | none => .absent
+    | some value => .present (local_type_correctness h ▸ value)
+
+namespace Network.Executable    
+
+def apply (exec : Executable net) (output : Reaction.Output net) : Executable net := { exec with
+  queue := exec.queue.merge output.events
+  reactors := fun id => { exec.reactors id with
+    interface := 
+      if      h : id = output.reactor then h ▸ targetReactor exec output  -- Updates the output ports of the reaction's reactor.
+      else if h : id ≻ output.reactor then nestedReactor exec output id h -- Updates the input ports of nested reactors.
+      else                                 exec.reactors id |>.interface  -- Unaffected reactors.
+  }
+  lawfulQueue := sorry
+}
+where 
+  targetReactor (exec : Executable net) (output : Reaction.Output net) : (kind : Reactor.InterfaceKind) → kind.interfaceType (output.reactor.class.interface kind)
+    | .outputs => fun var => (output.local var).value?.orElse (fun _ => exec.interface output.reactor .outputs var)
+    | .state => output.raw.state
+    | interface => exec.interface output.reactor interface
+  nestedReactor (exec : Executable net) (output : Reaction.Output net) (id : ReactorId net) (hc : id ≻ output.reactor) : (kind : Reactor.InterfaceKind) → kind.interfaceType (id.class.interface kind)
+    | .inputs => nestedInputs exec output id hc
+    | interface => exec.reactors id |>.interface interface 
+  nestedInputs (exec : Executable net) (output : Reaction.Output net) (id : ReactorId net) (hc : id ≻ output.reactor) : Interface? (id.class.interface .inputs) :=
+    let currentReactor := exec.reactors id
+    fun var =>
+      /-
+      let nestedID := id.last hc
+      have h₁ : (net.scheme id |>.interface .inputs).vars = (net.subinterface (net.class reactorID) nestedID .inputs).vars := by sorry -- rw [Graph.child_schemes_eq_parent_subschemes]
+      let var₁ : (net.reactionOutputScheme' reactorID).vars := .inr ⟨nestedID, h₁ ▸ var⟩
+      match h : InjectiveCoe.inv var₁ with 
+      | none => currentReactor.interface .inputs var
+      | some var₂ =>
+        match output.ports var₂ with
+        | none => currentReactor.interface .inputs var
+        | some val =>
+          have h : (net.class reactorID |> net.reactionOutputScheme |>.restrict reaction.portEffects).type var₂ = (net.scheme id |>.interface .inputs).type var := by
+            rw [(net.reactionOutputScheme' reactorID).restrict_type]
+            rw [InjectiveCoe.invCoeId _ h]
+            -- have := Graph.child_schemes_eq_parent_subschemes hc
+            sorry
+          h ▸ val
+      -/
+      sorry
+
+
+end Network.Executable    
